ask arthur line 89 of proofs_new

semantics/proofs_new.v
@@ -29,20 +29,65 @@ Admitted.
 Inductive all_diff_in_fw: nvmem -> vmem -> command -> nvmem -> Prop :=
   Diff_in_FW: forall{N1 V1 c1 N2 V2 c2 N1c O W} (T: trace_cs (N1, V1, c1) (N2, V2, c2) O W),
     end_com c2 -> checkpoint \notin O -> (*c2 is nearest checkpoint or termination*)
-    (getdomain N1) = (getdomain N2) -> (*alternatively
+    (getdomain N1) = (getdomain N1c) -> (*alternatively
                                        could check N2 domain as well instead of this*)
    (forall(el: el_loc), (inr el) \in (getdomain N1) -> ((getmap N1) (inr el)) = ((getmap N2) (inr el))) ->
 ( forall(l: loc ), l \in (getdomain N1) -> ((getmap N1) l <> (getmap N2) l) -> (l \in getfstwt W))
 -> all_diff_in_fw N1 V1 c1 N1c.
 
-Lemma two Ni Ni1 V V1 c c1 Nc Nc1 O W: all_diff_in_fw Ni V c Nc ->
+Lemma two {Ni Ni1 V V1 c c1 Nc O W} : all_diff_in_fw Ni V c Nc ->
                               cceval_w (Ni, V, c) O (Ni1, V1, c1) W ->
-                              (cceval_w (Nc, V, c) O (Nc1, V1, c1) W /\
+                              exists(Nc1: nvmem), (cceval_w (Nc, V, c) O (Nc1, V1, c1) W /\
                               forall(l: loc), l \in (getwt W) -> ((getmap Ni1) l = (getmap Nc1) l)).
 Admitted.
 
+Lemma empty_trace_s: forall{C1 C2: context} {O: obseq} {W: the_write_stuff},
+    trace_cs C1 C2 O W -> O = [::] -> C1 = C2 /\ W = emptysets.
+Admitted.
+
+Lemma observe_checkpt_s: forall {N N': nvmem} {V V': vmem}
+                     {c c' : command} {w: warvars}
+                    {O: obseq} {W: the_write_stuff},
+    cceval_w (N, V, (incheckpoint w ;; c)) O (N', V', c') W ->
+    checkpoint \in O. Admitted.
+
+Lemma single_step_alls: forall{C1 Cmid C3: context}
+                    {Obig: obseq} {Wbig: the_write_stuff},
+    trace_cs C1 C3 Obig Wbig ->
+    Obig <> [::] ->
+    (exists (O1: obseq) (W1: the_write_stuff), cceval_w C1 O1 Cmid W1) ->
+    exists(Wrest: the_write_stuff) (Orest: obseq), trace_c Cmid C3 Orest Wrest
+/\ subseq Orest Obig
+. Admitted.
+
 Lemma three N0 V0 c0 N01 V01 c01 Ni Ni1 V V1 c c1 Nc O W:
   all_diff_in_fw Ni V c Nc ->
-  trace_is ((N0, V0, c0), Ni, V, c) ((N01, V01, c01), Ni1, V1, c1) O W ->
+  trace_i1 ((N0, V0, c0), Ni, V, c) ((N01, V01, c01), Ni1, V1, c1) O W ->
   ( exists(Nc1: nvmem), trace_cs (Nc, V, c) (Nc1, V1, c1) O W /\
-  all_diff_in_fw Ni1 V1 c1 Nc1).
+                   all_diff_in_fw Ni1 V1 c1 Nc1).
+Proof.
+  intros. move: Nc H. dependent induction H0.
+  + dependent induction H; intros.
+    (*empty trace case*)
+  - exists Nc; split; auto; constructor.
+    (*cceval case*)
+  - move: (two H1 H) => [Nc1 [Hcceval Heq] ]. exists Nc1.
+    split. apply CsTrace_Single; assumption.
+    econstructor. inversion H1. subst.
+    (*getting ready to apply single_step_alls*)
+    assert (O0 <> [::]) as Ho0.
+    - move/ (empty_trace_s T) => [ [contra10 [contra11 contra12] ] contra2]. subst. case H2 as [Hskip | [crem [w Hcp] ] ]; subst.
+    inversion Hcceval. move/negP : H0. apply.
+    (*start here why is apply/negP different from this*)
+    apply (observe_checkpt_s Hcceval).
+    (*ask arthur i want to write
+     exists O exists W H, like a function*)
+    assert (exists(Oc: obseq) (Wc: the_write_stuff),
+               cceval_w (Ni, V, c) O (Ni1, V1, c1) W) as Hcceval2.
+    (*ask arthur why does it look like that*)
+    by exists O W. 
+    pose proof (single_step_alls T Ho0 Hcceval2).
+    move: (observe_checkpt_s Hcceval) => Hin. apply H3.
+    remember T as T1. apply (contra _ _ _) in T.
+    apply T.
+ -
